Language.v
@@ -1,0 +1,249 @@
+(**
+
+This file describes the syntax of an imperative lambda 
+calculus with records and arrays.
+
+Author: Ramon Fernandez I Mir and Arthur Charguéraud.
+
+License: MIT.
+
+*)
+
+Set Implicit Arguments.
+Require Export Bind TLCbuffer.
+Require Export LibString LibCore LibLogic LibReflect 
+  LibOption LibRelation LibLogic LibOperation LibEpsilon 
+  LibMonoid LibSet LibContainer LibList LibListZ LibMap.
+
+Open Scope set_scope.
+Open Scope container_scope.
+
+
+(* ********************************************************************** *)
+(* * Syntax *)
+
+(* ---------------------------------------------------------------------- *)
+(** Representation of locations and fields *)
+
+(** [loc] describes base pointers to an allocated block. *)
+
+Definition loc := nat. 
+
+Definition null : loc := 0%nat.
+
+Definition field := var.
+
+Definition size := nat.
+
+Definition offset := nat.
+
+Notation typvar := var.
+
+
+(* ---------------------------------------------------------------------- *)
+(** Grammar of types *)
+
+Inductive typ : Type :=
+  | typ_unit : typ
+  | typ_int : typ
+  | typ_double : typ
+  | typ_bool : typ
+  | typ_ptr : typ -> typ
+  | typ_array : typ -> option size -> typ
+  | typ_struct : map field typ -> typ
+  | typ_fun : list typ -> typ -> typ
+  | typ_var : typvar -> typ.
+
+Definition typdefctx := map typvar typ.
+
+
+(* ---------------------------------------------------------------------- *)
+(** Size of types *)
+
+Section TypeSizes.
+Open Scope nat_scope.
+
+Definition typdefctx_size := (map typvar size).
+
+Definition typdefctx_offset := (map typvar (map field offset)).
+
+(*Fixpoint sizeof (T:typ) : size := 
+  match T with
+  | typ_unit => 0
+  | typ_bool => 1
+  | typ_int => 1
+  | typ_double => 2
+  | typ_ptr _ => 1
+  | typ_array T' (Some n) => (n * (sizeof T'))
+  | typ_struct m => fold (monoid_make plus 0) (fun f T' => sizeof T') m
+  | typ_fun _ _ => 1
+  | _ => 0
+  end.*)
+
+End TypeSizes.
+
+
+(* ---------------------------------------------------------------------- *)
+(** Syntax of the source language *)
+
+Inductive access : Type :=
+  | access_array : typ -> int -> access
+  | access_field : typ -> field -> access.
+
+Definition accesses := list access. 
+
+Inductive binop : Type :=
+  | binop_eq : binop
+  | binop_sub : binop
+  | binop_add : binop
+  | binop_ptr_add : binop.
+
+Inductive prim : Type :=
+  | prim_binop : binop -> prim
+  | prim_get : typ -> prim
+  | prim_set : typ -> prim
+  | prim_new : typ -> prim
+  | prim_new_array : typ -> prim
+  | prim_struct_access : typ -> field -> prim
+  | prim_array_access : typ -> prim
+  | prim_struct_get : typ -> field -> prim
+  | prim_array_get : typ -> prim.
+
+(** TODO: Change this! Probably use Flocq? *)
+Definition double := int.
+
+Inductive val : Type :=
+  | val_error : val
+  | val_unit : val
+  | val_uninitialized : val
+  | val_bool : bool -> val
+  | val_int : int -> val
+  | val_double : double -> val
+  | val_abstract_ptr : loc -> accesses -> val
+  | val_concrete_ptr : loc -> offset -> val
+  | val_array : typ -> list val -> val
+  | val_struct : typ -> map field val -> val.
+
+Inductive trm : Type :=
+  | trm_var : var -> trm
+  | trm_val : val -> trm
+  | trm_if : trm -> trm -> trm -> trm
+  | trm_let : bind -> trm -> trm -> trm
+  | trm_app : prim -> list trm -> trm
+  | trm_while : trm -> trm -> trm
+  | trm_for : var -> val -> val -> trm -> trm.
+
+(** Sequence is a special case of let bindings *)
+
+Notation trm_seq := (trm_let bind_anon).
+
+(** Shorthand [vars], [vals] and [trms] for lists of items. *)
+
+Definition vals : Type := list val.
+Definition trms : Type := list trm.
+
+
+(* ---------------------------------------------------------------------- *)
+(** Inhabited types *)
+
+(** The type of values is inhabited *)
+
+Global Instance Inhab_val : Inhab val.
+Proof using. apply (Inhab_of_val val_unit). Qed.
+
+Global Instance Inhab_trm : Inhab trm.
+Proof using. apply (Inhab_of_val (trm_val val_unit)). Qed.
+
+Global Instance Inhab_typ : Inhab typ.
+Proof using. apply (Inhab_of_val typ_unit). Qed.
+
+Hint Extern 1 (Inhab val) => apply Inhab_val.
+
+Hint Extern 1 (Inhab typ) => apply Inhab_typ.
+
+
+(* ---------------------------------------------------------------------- *)
+(** Coercions *)
+
+Coercion prim_binop : binop >-> prim.
+Coercion val_int : Z >-> val.
+Coercion trm_val : val >-> trm.
+Coercion trm_var : var >-> trm.
+Coercion trm_app : prim >-> Funclass.
+
+
+(* ---------------------------------------------------------------------- *)
+(** Implicit types *)
+
+Implicit Types t : trm.
+Implicit Types v : val.
+Implicit Types l : loc.
+Implicit Types b : bool.
+Implicit Types x : var.
+Implicit Types z : bind.
+Implicit Types vs : vals.
+Implicit Types ts : trms.
+
+
+(* ---------------------------------------------------------------------- *)
+(** Auxiliary predicates for the semantics *)
+
+Definition is_val (t:trm) :=
+  match t with
+  | trm_val v => True
+  | _ => False
+  end.
+
+Definition is_error (v:val) :=
+  match v with
+  | val_error => True
+  | _ => False
+  end.
+
+Definition is_uninitialized (v:val) :=
+  match v with
+  | val_uninitialized => True
+  | _ => False
+  end.
+
+Definition is_bool (v:val) :=
+  match v with
+  | val_bool b => True
+  | _ => False
+  end.
+
+Definition is_ptr (v:val) :=
+  match v with
+  | val_abstract_ptr l π => True
+  | _ => False
+  end.
+
+Definition is_int (v:val) :=
+  match v with
+  | val_int i => True
+  | _ => False
+  end.
+
+Definition is_struct (v:val) :=
+  match v with
+  | val_struct T m => True
+  | _ => False
+  end.
+
+Definition is_array (v:val) :=
+  match v with
+  | val_array T a => True
+  | _ => False
+  end.
+
+
+(* ---------------------------------------------------------------------- *)
+(** State and stack *)
+
+(** Representation of the state *)
+
+Definition state := map loc val.
+
+(** Representation of the stack *)
+
+Definition stack := Ctx.ctx val.
